Fairness/All.v
@@ -1,8 +1,0 @@
-(* Fairness/All.v *)
-From Fairness Require Export PriorityFairness QuantityFairness MatchFinality Maximality RejectionFairness.
-(* Each of these files should expose the closed LTL formulas: *)
-(*   priorityOK : formula *)
-(*   allocOK    : formula *)
-(*   final      : formula *)
-(*   maximal    : formula *)
-(*   rejectionOK: formula *)
