Fairness/Fairness.v
@@ -1,0 +1,2 @@
+(* Fairness/Fairness.v *)
+From Fairness Require Export Interpretation PriorityFairness QuantityFairness MatchFinality Maximality RejectionFairness.
