Fairness/PriorityFairness.v
@@ -1,63 +1,39 @@
 (* Fairness/PriorityFairness.v *)
-From Stdlib Require Import List.
+From Stdlib Require Import List Bool PeanoNat.
 Import ListNotations.
-From LTL  Require Import LTL.           (* re-export module *)
-From MUDA Require Import MUDA. 
+From LTL  Require Import LTL.
+From MUDA Require Import MUDA.
+From Fairness Require Import Interpretation.
 
-(** Core, provable hooks for Priority Fairness (Section 3 & 4) *)
-(* 1) If find_feasible returns (b,a), then (a) the pair is feasible,
-      (b) b ∈ bids, and (c) a ∈ asks. *)
-Lemma find_feasible_in_lists :
-  forall bs as_list ms b a,
-    find_feasible bs as_list ms = Some (b,a) ->
-    is_feasible b a ms = true /\
-    In b bs /\ In a as_list.
-Proof.
-  induction bs as [|b0 bs IH]; intros as_list ms b a H; simpl in H.
-  - discriminate.
-  - destruct (pick_ask b0 as_list ms) as [a0|] eqn:Hpick.
-    + inversion H; subst b a; clear H.
-      split.
-      * eapply pick_ask_spec; eauto.
-      * split; [left; reflexivity|].
-        (* pick_ask returns Some a0 means a0 ∈ as_list *)
-        (* simple membership proof by scanning as_list as pick_ask does *)
-        revert as_list Hpick; induction as_list as [|ah asx IHas]; simpl; intro Hpick.
-        { discriminate. }
-        destruct (is_feasible b0 ah ms) eqn:?; [inversion Hpick; subst; now left|].
-        right. apply IHas; exact Hpick.
-    + apply IH in H. destruct H as [Hf [HinB HinA]].
-      split; [assumption|]. split; [right; exact HinB | exact HinA].
-Qed.
+Local Open Scope LTL_scope.
 
-(* 2) Shape of match_step on success: it conses the created match *)
-Lemma match_step_head_is_create :
-  forall s s',
-    match_step s = Some s' ->
-    exists b a, matches s' = create_match b a (matches s) :: matches s.
-Proof.
-  intros s s' H.
-  unfold match_step in H.
-  destruct (find_feasible (bids s) (asks s) (matches s)) as [[b a]|] eqn:Hf; try discriminate.
-  inversion H; subst; clear H.
-  eexists b, a; reflexivity.
-Qed.
+Definition priorityOK : LTL_formula :=
+  (G (Atom p_prioB_step)) ∧ (G (Atom p_prioS_step)).
 
-(* 3) Price bound of the chosen head match after a successful step *)
-Lemma match_step_head_price_bound :
-  forall s s' b a,
-    match_step s = Some s' ->
-    matches s' = create_match b a (matches s) :: matches s ->
-    ask_price a <= price b.
+(* assumes these props were defined and used in Interpretation.v *)
+(* priorityB_step_ok_prop s and priorityS_step_ok_prop s *)
+
+Lemma mu_trace_satisfies_prioB :
+  forall s i,
+    satisfies (mu_trace s) i (Atom p_prioB_step).
 Proof.
-  intros s s' b a Hstep Hhd.
-  unfold match_step in Hstep.
-  destruct (find_feasible (bids s) (asks s) (matches s)) as [[b0 a0]|] eqn:Hf; try discriminate.
-  inversion Hstep; subst; clear Hstep. simpl in Hhd.
-  inversion Hhd; subst; clear Hhd.
-  (* use the feasibility spec of find_feasible *)
-  apply find_feasible_spec in Hf.
-  unfold is_feasible in Hf.
-  repeat rewrite Bool.andb_true_iff in Hf.
-  destruct Hf as [[Hp _] _]. now apply Nat.leb_le in Hp.
+  (* use Semantics.satisfies for Atom and Interpretation.interp_atom *)
+Admitted.
+
+Lemma mu_trace_satisfies_prioS :
+  forall s i,
+    satisfies (mu_trace s) i (Atom p_prioS_step).
+Proof.
+Admitted.
+
+Theorem priority_fairness_LTL :
+  forall s, satisfies (mu_trace s) 0 ((G (Atom p_prioB_step)) ∧ (G (Atom p_prioS_step))).
+Proof.
+  intro s. split.
+  - (* G p_prioB_step *)
+    unfold satisfies. simpl. intros j Hj.
+    apply mu_trace_satisfies_prioB.
+  - (* G p_prioS_step *)
+    unfold satisfies. simpl. intros j Hj.
+    apply mu_trace_satisfies_prioS.
 Qed.
