LTL/LTL.v
@@ -1,4 +1,3 @@
 (* LTL/LTL.v *)
 From LTL Require Export Syntax Semantics Axioms Soundness Completeness.
 Local Open Scope LTL_scope.
-Export LTL.Completeness.
